src/theories/FOLTrees.v
@@ -94,6 +94,68 @@ Section Tree.
         )
       ).
   Proof. intros; exact eq_refl. Qed.
+
+
+  Fixpoint lt_t (k: Z) (t: tree) : Prop := 
+    match t with 
+    | Emp => True
+    | Node l k' _ r => (k' < k)%Z /\ lt_t k l /\ lt_t k r
+    end. 
+
+  Lemma lt_t_emp: 
+    forall k, 
+      lt_t k Emp.
+  Proof. intros; simpl; intuition. Qed.
+
+  Lemma lt_t_node: 
+    forall k l k' v r, 
+      (k' < k)%Z ->
+      lt_t k l -> 
+      lt_t k r -> 
+      lt_t k (Node l k' v r).
+  Proof. intros; simpl; intuition. Qed.
+
+  Fixpoint gt_t (k: Z) (t: tree) : Prop := 
+    match t with 
+    | Emp => True
+    | Node l k' _ r => (k' > k)%Z /\ gt_t k l /\ gt_t k r
+    end. 
+
+  Lemma gt_t_emp: 
+    forall k, 
+      gt_t k Emp.
+  Proof. intros; simpl; intuition. Qed.
+
+  Lemma gt_t_node: 
+    forall k l k' v r, 
+      (k' > k)%Z ->
+      gt_t k l -> 
+      gt_t k r -> 
+      gt_t k (Node l k' v r).
+  Proof. intros; simpl; intuition. Qed.
+
+  Fixpoint balanced (t: tree) : Prop :=
+    match t with 
+    | Emp => True
+    | Node l k _ r => 
+      lt_t k l /\ 
+      gt_t k r /\ 
+      balanced l /\ balanced r
+    end.
+  
+  Lemma balanced_emp: 
+    balanced Emp.
+  Proof. intros; simpl; intuition. Qed.
+
+  Lemma balanced_node: 
+    forall l k v r, 
+      balanced l -> 
+      balanced r ->
+      lt_t k l -> 
+      gt_t k r ->
+      balanced (Node l k v r).
+  Proof. intros; simpl; intuition. Qed.
+
 End Tree.
 
 Arguments Emp {_}.
@@ -101,6 +163,9 @@ Arguments Node {_} _ _ _ _.
 Arguments bound {_} _ _.
 Arguments lookup {_} _ _ _.
 Arguments insert {_} _ _ _.
+Arguments lt_t {_} _ _.
+Arguments gt_t {_} _ _.
+Arguments balanced {_} _.
 
 Section FOLTree.
 
@@ -117,11 +182,19 @@ Section FOLTree.
     | z_gt : funs [ZS; ZS] BS
     | e_f : funs [] TreeS
     | t_f : funs [TreeS; ZS; TS; TreeS] TreeS
+    | bound_f : funs [ZS; TreeS] BS
+    | lookup_f : funs [TS; ZS; TreeS] TS
+    | insert_f : funs [ZS; TS; TreeS] TreeS
     | cond_b : funs [BS; BS; BS] BS
     | cond_t : funs [BS; TS; TS] TS
     | cond_tree : funs [BS; TreeS; TreeS] TreeS. 
 
-  Inductive rels: arity sorts -> Type :=.
+  Inductive rels: arity sorts -> Type :=
+    | lt_z : rels [ZS; ZS]
+    | gt_z : rels [ZS; ZS]
+    | gt_t_r : rels [ZS; TreeS]
+    | lt_t_r : rels [ZS; TreeS]
+    | balanced_r : rels [TreeS].
 
   Definition sig: signature :=
     {| sig_sorts := sorts;
@@ -139,7 +212,7 @@ Section FOLTree.
     | BS => bool
     end.
 
-  Obligation Tactic := idtac.
+  Local Obligation Tactic := idtac.
   Equations 
     mod_fns params ret (f: sig_funs sig params ret) (args: HList.t mod_sorts params) 
     : mod_sorts ret :=
@@ -149,16 +222,24 @@ Section FOLTree.
       mod_fns _ _ z_gt (l ::: r ::: _) := (l >? r)%Z;
       mod_fns _ _ e_f _ := Emp;
       mod_fns _ _ t_f (l ::: k ::: v ::: r ::: _) := Node l k v r;
-      mod_fns _ _ cond_b (t ::: l ::: r ::: _) := ite t l r;
+      mod_fns _ _ bound_f (k ::: t ::: _) := bound k t;
+      mod_fns _ _ lookup_f (d ::: k ::: t ::: _) := lookup d k t;
+      mod_fns _ _ insert_f (k ::: v ::: t ::: _) := insert k v t;
       mod_fns _ _ cond_t (t ::: l ::: r ::: _) := ite t l r;
+      mod_fns _ _ cond_b (t ::: l ::: r ::: _) := ite t l r;
       mod_fns _ _ cond_tree (t ::: l ::: r ::: _) := ite t l r;
     }.
 
-  Definition mod_rels params
+  Equations mod_rels params
     (args: sig_rels sig params)
     (env: HList.t mod_sorts params) : Prop :=
-    match args with
-    end.
+    { 
+      mod_rels _ lt_z (l ::: r ::: _) := (l < r)%Z;
+      mod_rels _ gt_z (l ::: r ::: _) := (l > r)%Z;
+      mod_rels _ lt_t_r (k ::: t ::: _) := lt_t k t;
+      mod_rels _ gt_t_r (k ::: t ::: _) := gt_t k t;
+      mod_rels _ balanced_r (t ::: _) := balanced t;
+    }.
 
   Program Definition fm_model : model sig := {|
     FirstOrder.mod_sorts := mod_sorts;
